Add early instantiation

thys/Pi_Calculus/Pi_Transition.thy
@@ -1,7 +1,7 @@
-(* Here we instantiate the general enhanced rule induction to 
+(* Here we instantiate the general enhanced rule induction to
 the "early" pi-calculus transition system.
-the adjective refers to the fact that inputs are instantiated 
-at transition time (whereas a "late" semantics would 
+the adjective refers to the fact that inputs are instantiated
+at transition time (whereas a "late" semantics would
 have transitons with bound inputs)
  *)
 theory Pi_Transition
@@ -13,13 +13,13 @@ hide_const trans
 
 (* INSTANTIATING THE ABSTRACT SETTING: *)
 
-(* INSTATIATING THE Small LOCALE (INDEPENDENTLY OF THE CONSIDERED INDUCTIVE PREDICATE *) 
+(* INSTATIATING THE Small LOCALE (INDEPENDENTLY OF THE CONSIDERED INDUCTIVE PREDICATE *)
 
 print_locales
 
-(* The "late" transition relation  *)
+(* The "early" transition relation  *)
 inductive trans :: "trm \<Rightarrow> cmt \<Rightarrow> bool" where
-Inp: "\<comment> \<open>Present in Bengtson: x \<notin> {a,u} \<Longrightarrow> \<close>
+InpE: "\<comment> \<open>Present in Bengtson: x \<notin> {a,u} \<Longrightarrow> \<close>
 trans (Inp a x P) (Finp a u (usub P u x))"
 (* |
 Out: "trans (Out a x P) (Fout a x P)"
@@ -33,46 +33,46 @@ Sum1: "trans P1 C \<Longrightarrow> trans (Sum P1 P2) C"
 Sum2: "trans P2 C \<Longrightarrow> trans (Sum P1 P2) C"
 *)
 |
-Open: "trans P (Fout a x P') \<Longrightarrow> a \<noteq> x \<Longrightarrow> 
+Open: "trans P (Fout a x P') \<Longrightarrow> a \<noteq> x \<Longrightarrow>
        trans (Res x P) (Bout a x P')"
 |
-ScopeF: "trans P (Cmt act P') \<Longrightarrow> \<not> is_bout act \<Longrightarrow> x \<notin> vars act \<Longrightarrow> 
+ScopeFree: "trans P (Cmt act P') \<Longrightarrow> \<not> is_bout act \<Longrightarrow> x \<notin> vars act \<Longrightarrow>
    trans (Res x P) (Cmt act (Res x P'))"
 |
 ScopeB: "trans P (Bout a x P') \<Longrightarrow> y \<notin> {a,x} \<Longrightarrow> x \<notin> {a} \<union> FFVars P
-   \<Longrightarrow> 
+   \<Longrightarrow>
    trans (Res y P) (Bout a x (Res y P'))"
 |
-Par1: "trans P1 (Cmt act P1') \<Longrightarrow> 
-   \<^cancel>\<open>present in Bengtson but not needed (and will be an 'output' 
-      of strong induction) : bvars act \<inter> fvars act = {} \<Longrightarrow> \<close>  
-   bvars act \<inter> FFVars P1 = {} \<Longrightarrow> 
-   bvars act \<inter> FFVars P2 = {} \<Longrightarrow> 
-   trans (Par P1 P2) (Cmt act (Par P1' P2))" 
+Par1: "trans P1 (Cmt act P1') \<Longrightarrow>
+   \<^cancel>\<open>present in Bengtson but not needed (and will be an 'output'
+      of strong induction) : bvars act \<inter> fvars act = {} \<Longrightarrow> \<close>
+   bvars act \<inter> FFVars P1 = {} \<Longrightarrow>
+   bvars act \<inter> FFVars P2 = {} \<Longrightarrow>
+   trans (Par P1 P2) (Cmt act (Par P1' P2))"
 (* |
-Par2: "trans P2 (Cmt act P2') \<Longrightarrow> bvars act \<inter> FFVars P1 = {} \<Longrightarrow> 
+Par2: "trans P2 (Cmt act P2') \<Longrightarrow> bvars act \<inter> FFVars P1 = {} \<Longrightarrow>
    trans (Par P1 P2) (Cmt act (Par P1 P2'))" *)
 |
-Com1: "trans P1 (Finp a x P1') \<Longrightarrow> trans P2 (Fout a x P2') \<Longrightarrow> 
-   trans (Par P1 P2) (Tau (Par P1' P2'))" 
+Com1: "trans P1 (Finp a x P1') \<Longrightarrow> trans P2 (Fout a x P2') \<Longrightarrow>
+   trans (Par P1 P2) (Tau (Par P1' P2'))"
 (* |
-Com2: "trans P1 (Fout a x P1') \<Longrightarrow> trans P2 (Finp a x P2') \<Longrightarrow> 
+Com2: "trans P1 (Fout a x P1') \<Longrightarrow> trans P2 (Finp a x P2') \<Longrightarrow>
    trans (Par P1 P2) (Tau (Par P1' P2'))"  *)
 |
 Close1: "trans P1 (Finp a x P1') \<Longrightarrow> trans P2 (Bout a x  P2') \<Longrightarrow>
-    \<^cancel>\<open>  x \<noteq> a seems essential, and not an artifact \<close> 
+    \<^cancel>\<open>  x \<noteq> a seems essential, and not an artifact \<close>
    x \<notin> {a} \<union> FFVars P1 \<^cancel>\<open>\<union> FFVars P2 was in Bengtson\<close>  \<Longrightarrow>
-   trans (Par P1 P2) (Tau (Res x (Par P1' P2')))" 
-(*  
+   trans (Par P1 P2) (Tau (Res x (Par P1' P2')))"
+(*
 x fresh P1  x=/=a
-trans (P1=[xx/x]) (Finp a[xx/x[xx/x])] xx P1' \<Longrightarrow> trans P2 (Bout a xx  P2'[xx/x]) 
+trans (P1=[xx/x]) (Finp a[xx/x[xx/x])] xx P1' \<Longrightarrow> trans P2 (Bout a xx  P2'[xx/x])
 \<Longrightarrow>
-trans (Par P1 P2) (Bout a xx (Par P1'[xx/x] P2'[xx/x])) 
+trans (Par P1 P2) (Bout a xx (Par P1'[xx/x] P2'[xx/x]))
 *)
 (* |
-Close2: "trans P1 (Bout a x P1') \<Longrightarrow> trans P2 (Finp a x P2') \<Longrightarrow> 
+Close2: "trans P1 (Bout a x P1') \<Longrightarrow> trans P2 (Finp a x P2') \<Longrightarrow>
    x \<notin> {a} \<union> FFVars P1 \<union> FFVars P2 \<Longrightarrow>
-   trans (Par P1 P2) (Bout a x (Par P1' P2'))" 
+   trans (Par P1 P2) (Bout a x (Par P1' P2'))"
 |
 Bang: "trans (Par P (Bang P)) C \<Longrightarrow> trans (Bang P) C"
 *)
@@ -81,35 +81,35 @@ Bang: "trans (Par P (Bang P)) C \<Longrightarrow> trans (Bang P) C"
 (* INSTANTIATING THE LSNominalSet LOCALE: *)
 
 type_synonym T = "trm \<times> cmt"
-type_synonym V = "var list" 
+type_synonym V = "var list"
 
 
-definition Tperm :: "(var \<Rightarrow> var) \<Rightarrow> T \<Rightarrow> T" where 
+definition Tperm :: "(var \<Rightarrow> var) \<Rightarrow> T \<Rightarrow> T" where
 "Tperm f \<equiv> map_prod (rrename f) (rrename_commit f)"
 
-fun Tsupp :: "T \<Rightarrow> var set" where 
+fun Tsupp :: "T \<Rightarrow> var set" where
 "Tsupp (e1,e2) = FFVars e1 \<union> FFVars_commit e2"
 
 (*
-definition Vmap :: "(var \<Rightarrow> var) \<Rightarrow> V \<Rightarrow> V" where 
+definition Vmap :: "(var \<Rightarrow> var) \<Rightarrow> V \<Rightarrow> V" where
 "Vmap \<equiv> map"
 
-fun Vfvars :: "V \<Rightarrow> var set" where 
+fun Vfvars :: "V \<Rightarrow> var set" where
 "Vfvars v = set v"
 *)
 
 lemmas commit_internal.FFVars_rrenames[simp]
 
-interpretation LSNominalSet where 
+interpretation LSNominalSet where
 Tperm = Tperm and Tsupp = Tsupp
-apply standard unfolding isPerm_def Tperm_def 
+apply standard unfolding isPerm_def Tperm_def
   using small_Un small_def term.card_of_FFVars_bounds
     commit_internal.card_of_FFVars_bounds(2)
-  apply (auto simp: term.rrename_id0s map_prod.comp term.rrename_comp0s 
+  apply (auto simp: term.rrename_id0s map_prod.comp term.rrename_comp0s
         commit_internal.rrename_cong_ids(2)
         commit_internal.rrename_id0s commit_internal.rrename_comp0s(2)
-          infinite_UNIV) 
-  by blast 
+          infinite_UNIV)
+  by blast
 
 lemma small_bvars[simp,intro!]: "small (bvars act)"
 by (cases act, auto)
@@ -117,39 +117,39 @@ by (cases act, auto)
 definition G :: "var set \<Rightarrow> (T \<Rightarrow> bool) \<Rightarrow> T \<Rightarrow> bool"
 where
 "G \<equiv> \<lambda>B R t.
- \<^cancel>\<open>Inp: \<close>  
- (\<exists>x a u P. 
-    B = {x} \<and> fst t = Inp a x P \<and> snd t = Finp a u (usub P u x) 
+ \<^cancel>\<open>Inp: \<close>
+ (\<exists>x a u P.
+    B = {x} \<and> fst t = Inp a x P \<and> snd t = Finp a u (usub P u x)
  \<comment> \<open>\<and> x \<notin> {a,u} \<close>)
- \<or>  \<^cancel>\<open>Open: \<close> 
- (\<exists>P a x P'. 
-    B = {x} \<and> fst t = Res x P \<and> snd t = Bout a x P' \<and> 
-    a \<noteq> x \<and> 
-    R (P,Fout a x P')) 
- \<or>  \<^cancel>\<open>ScopeF: \<close> 
- (\<exists> P act P' x.  
-    B = {x} \<and> fst t = Res x P \<and> snd t = Cmt act (Res x P') \<and>  
-    \<not> is_bout act \<and> x \<notin> vars act \<and> 
+ \<or>  \<^cancel>\<open>Open: \<close>
+ (\<exists>P a x P'.
+    B = {x} \<and> fst t = Res x P \<and> snd t = Bout a x P' \<and>
+    a \<noteq> x \<and>
+    R (P,Fout a x P'))
+ \<or>  \<^cancel>\<open>ScopeF: \<close>
+ (\<exists> P act P' x.
+    B = {x} \<and> fst t = Res x P \<and> snd t = Cmt act (Res x P') \<and>
+    \<not> is_bout act \<and> x \<notin> vars act \<and>
     R (P, Cmt act P'))
- \<or>  \<^cancel>\<open>ScopeB: \<close> 
- (\<exists> P a x P' y. 
-    B = {x,y} \<and> fst t = Res y P \<and> snd t = Bout a x (Res y P') \<and>  
-    y \<notin> {a,x} \<and> x \<notin> {a} \<union> FFVars P \<and>  
+ \<or>  \<^cancel>\<open>ScopeB: \<close>
+ (\<exists> P a x P' y.
+    B = {x,y} \<and> fst t = Res y P \<and> snd t = Bout a x (Res y P') \<and>
+    y \<notin> {a,x} \<and> x \<notin> {a} \<union> FFVars P \<and>
     R (P, Bout a x P'))
- \<or>  \<^cancel>\<open>Par1: \<close> 
- (\<exists>P1 act P1' P2. 
-    B = bvars act \<and> fst t = Par P1 P2 \<and> snd t = Cmt act (Par P1' P2) \<and> 
-    bvars act \<inter> FFVars P1 = {} \<and> 
-    bvars act \<inter> FFVars P2 = {} \<and> 
+ \<or>  \<^cancel>\<open>Par1: \<close>
+ (\<exists>P1 act P1' P2.
+    B = bvars act \<and> fst t = Par P1 P2 \<and> snd t = Cmt act (Par P1' P2) \<and>
+    bvars act \<inter> FFVars P1 = {} \<and>
+    bvars act \<inter> FFVars P2 = {} \<and>
     R (P1, Cmt act P1'))
- \<or> \<^cancel>\<open>Com1: \<close> 
- (\<exists>P1 a x P1' P2 P2'. 
-    B = {} \<and> fst t = Par P1 P2 \<and> snd t = Tau (Par P1' P2') \<and>  
+ \<or> \<^cancel>\<open>Com1: \<close>
+ (\<exists>P1 a x P1' P2 P2'.
+    B = {} \<and> fst t = Par P1 P2 \<and> snd t = Tau (Par P1' P2') \<and>
     R (P1, Finp a x P1') \<and> R (P2, Fout a x P2'))
- \<or> \<^cancel>\<open>Close1: \<close> 
- (\<exists>P1 a x P1' P2 P2'. 
-    B = {x} \<and> fst t = Par P1 P2 \<and> snd t = Tau (Res x (Par P1' P2')) \<and> 
-    x \<notin> {a} \<union> FFVars P1 \<and> 
+ \<or> \<^cancel>\<open>Close1: \<close>
+ (\<exists>P1 a x P1' P2 P2'.
+    B = {x} \<and> fst t = Par P1 P2 \<and> snd t = Tau (Res x (Par P1' P2')) \<and>
+    x \<notin> {a} \<union> FFVars P1 \<and>
     R (P1, Finp a x P1') \<and> R (P2, Bout a x P2'))
 "
 
@@ -163,7 +163,7 @@ unfolding G_def by (smt (z3) le_boolE le_funD)
 (* *)
 
 (* lemma FFVars_commit_Cmt[simp]: "FFVars_commit (Cmt act P) = FFVars P" *)
- 
+
 
 (* NB: Everything is passed \<sigma>-renamed as witnesses to exI *)
 lemma GG_equiv: "isPerm \<sigma> \<Longrightarrow> small B \<Longrightarrow> G B R t \<Longrightarrow> G (image \<sigma> B) (\<lambda>t'. R (Tperm (inv \<sigma>) t')) (Tperm \<sigma> t)"
@@ -180,38 +180,38 @@ lemma GG_equiv: "isPerm \<sigma> \<Longrightarrow> small B \<Longrightarrow> G B
   (* Inp: *)
   subgoal apply(rule disjI7_1)
   subgoal apply(elim exE) subgoal for x a u P
-  apply(rule exI[of _ "\<sigma> x"]) apply(rule exI[of _ "\<sigma> a"]) 
+  apply(rule exI[of _ "\<sigma> x"]) apply(rule exI[of _ "\<sigma> a"])
   apply(rule exI[of _ "\<sigma> u"]) apply(rule exI[of _ "rrename \<sigma> P"])
-  apply(cases t) unfolding isPerm_def small_def Tperm_def 
-  by (simp add: term.rrename_comps) . . 
+  apply(cases t) unfolding isPerm_def small_def Tperm_def
+  by (simp add: term.rrename_comps) . .
   (* Open: *)
   subgoal apply(rule disjI7_2)
   subgoal apply(elim exE) subgoal for P a x P'
   apply(rule exI[of _ "rrename \<sigma> P"])
   apply(rule exI[of _ "\<sigma> a"]) apply(rule exI[of _ "\<sigma> x"])
-  apply(rule exI[of _ "rrename \<sigma> P'"])   
-  apply(cases t) unfolding isPerm_def small_def Tperm_def 
-  by (simp add: term.rrename_comps) . . 
+  apply(rule exI[of _ "rrename \<sigma> P'"])
+  apply(cases t) unfolding isPerm_def small_def Tperm_def
+  by (simp add: term.rrename_comps) . .
   (* ScopeF: *)
   subgoal apply(rule disjI7_3)
   subgoal apply(elim exE) subgoal for P act P' x
   apply(rule exI[of _ "rrename \<sigma> P"])
   apply(rule exI[of _ "map_action \<sigma> act"])
   apply(rule exI[of _ "rrename \<sigma> P'"])
-  apply(rule exI[of _ "\<sigma> x"]) 
-  apply(cases t) unfolding isPerm_def small_def Tperm_def  
-  apply (simp add: term.rrename_comps) 
+  apply(rule exI[of _ "\<sigma> x"])
+  apply(cases t) unfolding isPerm_def small_def Tperm_def
+  apply (simp add: term.rrename_comps)
   by (auto simp add: action.map_id action.map_comp) . .
   (* ScopeB: *)
   subgoal apply(rule disjI7_4)
   subgoal apply(elim exE) subgoal for P a x P' y
   apply(rule exI[of _ "rrename \<sigma> P"])
-  apply(rule exI[of _ "\<sigma> a"]) 
-  apply(rule exI[of _ "\<sigma> x"]) 
+  apply(rule exI[of _ "\<sigma> a"])
+  apply(rule exI[of _ "\<sigma> x"])
   apply(rule exI[of _ "rrename \<sigma> P'"])
-  apply(rule exI[of _ "\<sigma> y"])   
-  apply(cases t) unfolding isPerm_def small_def Tperm_def 
-  apply (simp add: term.rrename_comps) 
+  apply(rule exI[of _ "\<sigma> y"])
+  apply(cases t) unfolding isPerm_def small_def Tperm_def
+  apply (simp add: term.rrename_comps)
   by auto . .
   (* Par1: *)
   subgoal apply(rule disjI7_5)
@@ -220,8 +220,8 @@ lemma GG_equiv: "isPerm \<sigma> \<Longrightarrow> small B \<Longrightarrow> G B
   apply(rule exI[of _ "map_action \<sigma> act"])
   apply(rule exI[of _ "rrename \<sigma> P1'"])
   apply(rule exI[of _ "rrename \<sigma> P2"])
-  apply(cases t) unfolding isPerm_def small_def Tperm_def 
-  apply (simp add: term.rrename_comps)  
+  apply(cases t) unfolding isPerm_def small_def Tperm_def
+  apply (simp add: term.rrename_comps)
   by (auto simp add: action.map_id action.map_comp) . .
   (* Com1: *)
   subgoal apply(rule disjI7_6)
@@ -232,7 +232,7 @@ lemma GG_equiv: "isPerm \<sigma> \<Longrightarrow> small B \<Longrightarrow> G B
   apply(rule exI[of _ "rrename \<sigma> P1'"])
   apply(rule exI[of _ "rrename \<sigma> P2"])
   apply(rule exI[of _ "rrename \<sigma> P2'"])
-  apply(cases t) unfolding isPerm_def small_def Tperm_def 
+  apply(cases t) unfolding isPerm_def small_def Tperm_def
   by (simp add: term.rrename_comps) . .
   (* Close1: *)
   subgoal apply(rule disjI7_7)
@@ -243,7 +243,7 @@ lemma GG_equiv: "isPerm \<sigma> \<Longrightarrow> small B \<Longrightarrow> G B
   apply(rule exI[of _ "rrename \<sigma> P1'"])
   apply(rule exI[of _ "rrename \<sigma> P2"])
   apply(rule exI[of _ "rrename \<sigma> P2'"])
-  apply(cases t) unfolding isPerm_def small_def Tperm_def 
+  apply(cases t) unfolding isPerm_def small_def Tperm_def
   apply (simp add: term.rrename_comps)
   by auto . . .
 *)
@@ -265,11 +265,11 @@ using finite_iff_le_card_var small_Tsupp small_def by blast
 lemma exists_fresh:
 "\<exists> z. z \<notin> set xs \<and> (\<forall>t \<in> set ts. z \<notin> Tsupp t)"
 proof-
-  have 0: "|set xs \<union> \<Union> (Tsupp ` (set ts))| <o |UNIV::var set|" 
-  unfolding ls_UNIV_iff_finite  
+  have 0: "|set xs \<union> \<Union> (Tsupp ` (set ts))| <o |UNIV::var set|"
+  unfolding ls_UNIV_iff_finite
   using finite_Tsupp by blast
   then obtain x where "x \<notin> set xs \<union> \<Union> (Tsupp ` (set ts))"
-  by (meson ex_new_if_finite finite_iff_le_card_var 
+  by (meson ex_new_if_finite finite_iff_le_card_var
     infinite_iff_natLeq_ordLeq var_term_pre_class.large)
   thus ?thesis by auto
 qed
@@ -280,11 +280,11 @@ lemma finite_vars: "finite (vars act)"
 lemma exists_fresh':
 "\<exists> z. z \<notin> set xs \<and> (\<forall>t \<in> set as. z \<notin> vars t) \<and> (\<forall>t \<in> set ts. z \<notin> Tsupp t)"
 proof-
-  have 0: "|set xs \<union> \<Union> (Tsupp ` (set ts)) \<union> \<Union> (vars ` (set as))| <o |UNIV::var set|" 
+  have 0: "|set xs \<union> \<Union> (Tsupp ` (set ts)) \<union> \<Union> (vars ` (set as))| <o |UNIV::var set|"
   unfolding ls_UNIV_iff_finite
   using finite_Tsupp finite_vars by blast
   then obtain x where "x \<notin> set xs \<union> \<Union> (Tsupp ` (set ts)) \<union> \<Union> (vars ` (set as))"
-  by (meson ex_new_if_finite finite_iff_le_card_var 
+  by (meson ex_new_if_finite finite_iff_le_card_var
     infinite_iff_natLeq_ordLeq var_term_pre_class.large)
   thus ?thesis by auto
 qed
@@ -325,11 +325,11 @@ lemma swapa_idle: "xx \<notin> vars act \<Longrightarrow> x \<notin> vars act \<
 
 lemmas act_var_simps = not_is_bout_bvars empty_bvars_vars_fvars bvars_swapa fvars_swapa swapa_idle
 
-(* NB: The entities affected by variables are passed as witnesses to exI 
-with x and (the fresh) xx swapped, whereas the non-affected ones are passed 
-as they are. 
+(* NB: The entities affected by variables are passed as witnesses to exI
+with x and (the fresh) xx swapped, whereas the non-affected ones are passed
+as they are.
 *)
-lemma G_refresh: 
+lemma G_refresh:
   assumes "(\<forall>\<sigma> t. isPerm \<sigma> \<and> R t \<longrightarrow> R (Tperm \<sigma> t))"
   shows "small B \<Longrightarrow> G B R t \<Longrightarrow> \<exists>C. small C \<and> C \<inter> Tsupp t = {} \<and> G C R t"
 unfolding G_def
@@ -405,40 +405,40 @@ unfolding G_def
 (*
   using assms
 unfolding G_def Tperm_def apply(elim disjE exE conjE)
-  (* Inp: *) 
+  (* Inp: *)
   subgoal for x a u P
   using exists_fresh[of "[]" "[t]"] apply(elim exE conjE)
   subgoal for xx
-  apply(rule exI[of _ "{xx}"])  
+  apply(rule exI[of _ "{xx}"])
   apply(intro conjI)
     subgoal by simp
-    subgoal unfolding isPerm_def small_def by auto 
-    subgoal apply(rule disjI7_1) 
-    apply(rule exI[of _ "xx"]) 
+    subgoal unfolding isPerm_def small_def by auto
+    subgoal apply(rule disjI7_1)
+    apply(rule exI[of _ "xx"])
     apply(rule exI[of _ "a"])
-    apply(rule exI[of _ "u"]) 
+    apply(rule exI[of _ "u"])
     apply(rule exI[of _ "swap P x xx"])
-    apply(cases t) 
+    apply(cases t)
     by (simp add: Inp_refresh usub_refresh) . .
   (* Open: *)
   subgoal for P a x P'
   using exists_fresh[of "[]" "[t]"] apply(elim exE conjE)
   subgoal for xx
-  apply(rule exI[of _ "{xx}"])  
+  apply(rule exI[of _ "{xx}"])
   apply(intro conjI)
     subgoal by simp
-    subgoal unfolding isPerm_def small_def by auto 
-    subgoal apply(rule disjI7_2) 
+    subgoal unfolding isPerm_def small_def by auto
+    subgoal apply(rule disjI7_2)
     apply(rule exI[of _ "swap P x xx"])
-    apply(rule exI[of _ "a"]) 
+    apply(rule exI[of _ "a"])
     apply(rule exI[of _ "xx"])
-    apply(rule exI[of _ "swap P' x xx"]) 
+    apply(rule exI[of _ "swap P' x xx"])
     apply(cases t)  apply simp apply(intro conjI)
       subgoal using Res_refresh by blast
       subgoal by auto
       apply(erule allE[of _ "id(x:=xx,xx:=x)"])
       apply(erule allE[of _ "P"])
-      apply(erule allE[of _ "Fout a x P'"]) 
+      apply(erule allE[of _ "Fout a x P'"])
       by (auto simp: isPerm_def split: if_splits ) . .
   (* ScopeF: *)
   subgoal for P act P' x
@@ -446,49 +446,49 @@ unfolding G_def Tperm_def apply(elim disjE exE conjE)
     subgoal
     using exists_fresh[of "[]" "[t]"] apply(elim exE conjE)
     subgoal for xx
-    apply(rule exI[of _ "{xx}"])  
+    apply(rule exI[of _ "{xx}"])
     apply(intro conjI)
       subgoal by simp
-      subgoal unfolding isPerm_def small_def by auto 
-      subgoal apply(rule disjI7_3) 
+      subgoal unfolding isPerm_def small_def by auto
+      subgoal apply(rule disjI7_3)
       apply(rule exI[of _ "swap P x xx"])
-      apply(rule exI[of _ "swapa act x xx"]) 
+      apply(rule exI[of _ "swapa act x xx"])
       apply(rule exI[of _ "swap P' x xx"])
-      apply(rule exI[of _ "xx"]) 
+      apply(rule exI[of _ "xx"])
       apply(cases t) apply simp apply(intro conjI)
         subgoal using Res_refresh by blast
-        subgoal using Res_refresh apply(cases act, simp_all split: if_splits)  
+        subgoal using Res_refresh apply(cases act, simp_all split: if_splits)
         by blast+
         subgoal by auto
         subgoal apply(erule allE[of _ "id(x:=xx,xx:=x)"])
         apply(erule allE[of _ "P"])
-        apply(erule allE[of _ "Cmt act P'"]) 
+        apply(erule allE[of _ "Cmt act P'"])
         by (auto simp: isPerm_def split: if_splits ) . . . .
   (* ScopeB: *)
   subgoal for P a x P' y
   using exists_fresh[of "[a,x,y]" "[t]"] apply(elim exE conjE)
   subgoal for yy
   using exists_fresh[of "[a,x,y,yy]" "[t]"] apply(elim exE conjE)
-  subgoal for xx  
-  apply(rule exI[of _ "{xx,yy}"])  
+  subgoal for xx
+  apply(rule exI[of _ "{xx,yy}"])
   apply(intro conjI)
     subgoal by simp
-    subgoal unfolding isPerm_def small_def  by auto 
+    subgoal unfolding isPerm_def small_def  by auto
     subgoal apply(rule disjI7_4)
     apply(rule exI[of _ "swap P y yy"])
-    apply(rule exI[of _ "a"]) 
+    apply(rule exI[of _ "a"])
     apply(rule exI[of _ "xx"])
-    apply(rule exI[of _ "swap (swap P' x xx) y yy"]) 
+    apply(rule exI[of _ "swap (swap P' x xx) y yy"])
     apply(cases t) apply (simp add: sw_def) apply(intro conjI)
       subgoal using Res_refresh by auto
       apply(erule allE[of _ "id(x:=xx,xx:=x) o id(y:=yy,yy:=y)"])
       apply(erule allE[of _ "P"])
-      apply(erule allE[of _ "Bout a x P'"]) 
-      apply clarify apply(rule exI[of _ yy])     
+      apply(erule allE[of _ "Bout a x P'"])
+      apply clarify apply(rule exI[of _ yy])
       apply (simp add: isPerm_def rrename_o_swap split: if_splits)
-      apply safe 
+      apply safe
         subgoal using infinite_var not_ordLeq_ordLess supp_comp_bound by blast
-        subgoal by (metis (no_types, lifting) Res_inject_swap Res_refresh) 
+        subgoal by (metis (no_types, lifting) Res_inject_swap Res_refresh)
         subgoal using not_ordLess_ordLeq term_pre.supp_comp_bound by blast
         subgoal using Res_refresh by blast
         subgoal by (metis Res_inject_swap Res_refresh)
@@ -501,70 +501,70 @@ unfolding G_def Tperm_def apply(elim disjE exE conjE)
     subgoal
     using exists_fresh[of "[]" "[t]"] apply(elim exE conjE)
     subgoal for yy
-    apply(rule exI[of _ "{}"])  
+    apply(rule exI[of _ "{}"])
     apply(intro conjI)
       subgoal by simp
-      subgoal unfolding isPerm_def small_def by auto 
-      subgoal apply(rule disjI7_5) 
+      subgoal unfolding isPerm_def small_def by auto
+      subgoal apply(rule disjI7_5)
       apply(rule exI[of _ P1])
-      apply(rule exI[of _ act]) 
+      apply(rule exI[of _ act])
       apply(rule exI[of _ P1'])
-      apply(rule exI[of _ P2]) 
-      apply(cases t) by simp  . . 
+      apply(rule exI[of _ P2])
+      apply(cases t) by simp  . .
     (* *)
     subgoal for a b
     using exists_fresh[of "[a,b]" "[t]"] apply(elim exE conjE)
     subgoal for bb
-    apply(rule exI[of _ "{bb}"])  
+    apply(rule exI[of _ "{bb}"])
     apply(intro conjI)
       subgoal by simp
-      subgoal unfolding isPerm_def small_def by auto 
+      subgoal unfolding isPerm_def small_def by auto
       subgoal apply(rule disjI7_5)
-      apply(rule exI[of _ P1]) 
-      apply(rule exI[of _ "bout a bb"]) 
+      apply(rule exI[of _ P1])
+      apply(rule exI[of _ "bout a bb"])
       apply(rule exI[of _ "swap P1' b bb"])
-      apply(rule exI[of _ P2]) 
-      apply(cases t) apply simp  
-      by (metis Bout_inj) . . . 
+      apply(rule exI[of _ P2])
+      apply(cases t) apply simp
+      by (metis Bout_inj) . . .
   (* Com1: *)
   subgoal for P1 a x P1' P2 P2'
-  apply(rule exI[of _ "{}"])  
+  apply(rule exI[of _ "{}"])
   apply(intro conjI)
     subgoal by simp
-    subgoal unfolding isPerm_def small_def by auto 
-    subgoal apply(rule disjI7_6) 
+    subgoal unfolding isPerm_def small_def by auto
+    subgoal apply(rule disjI7_6)
       apply(rule exI[of _ P1])
-      apply(rule exI[of _ a]) 
+      apply(rule exI[of _ a])
       apply(rule exI[of _ x])
-      apply(rule exI[of _ P1']) 
-      apply(rule exI[of _ P2]) 
-      apply(rule exI[of _ P2']) 
-      apply(cases t) by simp . 
+      apply(rule exI[of _ P1'])
+      apply(rule exI[of _ P2])
+      apply(rule exI[of _ P2'])
+      apply(cases t) by simp .
   (* Close1: *)
   subgoal for P1 a x P1' P2 P2'
   using exists_fresh[of "[a,x]" "[t]"] apply(elim exE conjE)
   subgoal for xx
-  apply(rule exI[of _ "{xx}"])  
+  apply(rule exI[of _ "{xx}"])
   apply(intro conjI)
     subgoal by simp
-    subgoal unfolding isPerm_def small_def by auto 
+    subgoal unfolding isPerm_def small_def by auto
     subgoal apply(rule disjI7_7)
-    apply(rule exI[of _ "swap P1 x xx"]) 
-    apply(rule exI[of _ a]) 
+    apply(rule exI[of _ "swap P1 x xx"])
+    apply(rule exI[of _ a])
     apply(rule exI[of _ xx])
     apply(rule exI[of _ "swap P1' x xx"])
-    apply(rule exI[of _ P2]) 
-    apply(rule exI[of _ "swap P2' x xx"]) 
+    apply(rule exI[of _ P2])
+    apply(rule exI[of _ "swap P2' x xx"])
     apply(cases t) apply simp apply(intro conjI)
       subgoal by (simp add: Res_inject_swap fun_upd_twist)
       subgoal apply(erule allE[of _ "id(x:=xx,xx:=x)"])
       apply(erule allE[of _ "P1"])
-      apply(erule allE[of _ "Finp a x P1'"])      
-      by (auto simp: isPerm_def split: if_splits)  
+      apply(erule allE[of _ "Finp a x P1'"])
+      by (auto simp: isPerm_def split: if_splits)
       subgoal apply(erule allE[of _ "id(x:=xx,xx:=x)"])
       apply(erule allE[of _ "P1"])
-      apply(erule allE[of _ "Bout a x P1'"])      
-      apply (simp add: isPerm_def split: if_splits)  
+      apply(erule allE[of _ "Bout a x P1'"])
+      apply (simp add: isPerm_def split: if_splits)
       by (metis Bout_inj)+ . . .
 *) .
 
@@ -572,11 +572,11 @@ unfolding G_def Tperm_def apply(elim disjE exE conjE)
 
 interpretation Trans: Induct where
 Tperm = Tperm and Tsupp = Tsupp and G = G
-apply standard 
+apply standard
   using GG_mono GG_equiv G_refresh by auto
 
 
-lemma trans_I: "trans t1 t2 = Trans.I (t1,t2)" 
+lemma trans_I: "trans t1 t2 = Trans.I (t1,t2)"
 unfolding trans_def Trans.I_def lfp_curry2 apply(rule arg_cong2[of _ _ _ _ lfp], simp_all)
 unfolding fun_eq_iff G_def apply clarify
 subgoal for R PP QQ apply(rule iffI)
@@ -585,18 +585,18 @@ subgoal for R PP QQ apply(rule iffI)
     subgoal for a x P apply(rule exI[of _ "{x}"], rule conjI, simp) apply(rule disjI7_1) by auto
     \<^cancel>\<open>Open: \<close>
     subgoal for P a x apply(rule exI[of _ "{x}"], rule conjI, simp) apply(rule disjI7_2) by auto
-    \<^cancel>\<open>ScopeF: \<close> 
+    \<^cancel>\<open>ScopeF: \<close>
     subgoal for P act P' x apply(rule exI[of _ "{x}"], rule conjI, simp) apply(rule disjI7_3) by auto
-    \<^cancel>\<open>ScopeB: \<close> 
-    subgoal for P a x P' y 
-    apply(rule exI[of _ "{x, y}"], rule conjI, simp) apply(rule disjI7_4) 
+    \<^cancel>\<open>ScopeB: \<close>
+    subgoal for P a x P' y
+    apply(rule exI[of _ "{x, y}"], rule conjI, simp) apply(rule disjI7_4)
     by (fastforce simp: sw_def)
     \<^cancel>\<open>Par1: \<close>
-    subgoal for P1 act P1' P2 apply(rule exI[of _ "bvars act"], rule conjI, simp) 
+    subgoal for P1 act P1' P2 apply(rule exI[of _ "bvars act"], rule conjI, simp)
     apply(rule disjI7_5) by auto
-    \<^cancel>\<open>Com1: \<close> 
+    \<^cancel>\<open>Com1: \<close>
     subgoal for P1 a x P1' P2 apply(rule exI[of _ "{}"], rule conjI, simp) apply(rule disjI7_6) by auto
-    \<^cancel>\<open>Close1: \<close> 
+    \<^cancel>\<open>Close1: \<close>
     subgoal for P1 a x P1' P2 apply(rule exI[of _ "{x}"], rule conjI, simp) apply(rule disjI7_7) by auto .
     (* *)
   subgoal apply(elim conjE disjE exE)
@@ -604,71 +604,71 @@ subgoal for R PP QQ apply(rule iffI)
     subgoal apply(rule disjI7_1) by auto
     \<^cancel>\<open>Open: \<close>
     subgoal apply(rule disjI7_2) by fastforce
-    \<^cancel>\<open>ScopeF: \<close> 
+    \<^cancel>\<open>ScopeF: \<close>
     subgoal apply(rule disjI7_3) by auto
-    \<^cancel>\<open>ScopeB: \<close> 
+    \<^cancel>\<open>ScopeB: \<close>
     subgoal apply(rule disjI7_4) by (fastforce simp: sw_def)
     \<^cancel>\<open>Par1: \<close>
     subgoal apply(rule disjI7_5) by auto
-    \<^cancel>\<open>Com1: \<close> 
+    \<^cancel>\<open>Com1: \<close>
     subgoal apply(rule disjI7_6) by auto
-    \<^cancel>\<open>Close1: \<close> 
+    \<^cancel>\<open>Close1: \<close>
     subgoal apply(rule disjI7_7) by auto . . .
 
 (* FROM ABSTRACT BACK TO CONCRETE: *)
 thm trans.induct[of P C \<phi>, no_vars]
 
-corollary strong_induct_trans[consumes 2, case_names Inp Open ScopeF ScopeB Par1 Com1 Close1]: 
-assumes 
-par: "\<And>p. small (Psupp p)" 
+corollary strong_induct_trans[consumes 2, case_names Inp Open ScopeF ScopeB Par1 Com1 Close1]:
+assumes
+par: "\<And>p. small (Psupp p)"
 and tr: "trans P C"
-and Inp: 
-"\<And>x a u P p. x \<notin> {a, u} \<Longrightarrow> 
+and Inp:
+"\<And>x a u P p. x \<notin> {a, u} \<Longrightarrow>
     \<phi> p (Inp a x P) (Finp a u (usub P u x))"
-and Open:  
-"\<And>P a x P' p. x \<notin> Psupp p \<Longrightarrow> x \<noteq> a \<Longrightarrow> 
-    trans P (Fout a x P') \<Longrightarrow> (\<forall>p'. \<phi> p' P (Fout a x P')) \<Longrightarrow> a \<noteq> x \<Longrightarrow> 
+and Open:
+"\<And>P a x P' p. x \<notin> Psupp p \<Longrightarrow> x \<noteq> a \<Longrightarrow>
+    trans P (Fout a x P') \<Longrightarrow> (\<forall>p'. \<phi> p' P (Fout a x P')) \<Longrightarrow> a \<noteq> x \<Longrightarrow>
     \<phi> p (Res x P) (Bout a x P')"
-and ScopeF: 
-"\<And>P act P' y p. y \<notin> Psupp p \<Longrightarrow> y \<notin> fvars act \<Longrightarrow> 
-    trans P (Cmt act P') \<Longrightarrow> (\<forall>p'. \<phi> p' P (Cmt act P')) \<Longrightarrow> y \<notin> vars act \<Longrightarrow> 
+and ScopeF:
+"\<And>P act P' y p. y \<notin> Psupp p \<Longrightarrow> y \<notin> fvars act \<Longrightarrow>
+    trans P (Cmt act P') \<Longrightarrow> (\<forall>p'. \<phi> p' P (Cmt act P')) \<Longrightarrow> y \<notin> vars act \<Longrightarrow>
     \<phi> p (Res y P) (Cmt act (Res y P'))"
-and ScopeB: 
-"\<And>P a x P' y p. {x,y} \<inter> Psupp p = {} \<Longrightarrow> a \<notin> {x,y} \<Longrightarrow> 
+and ScopeB:
+"\<And>P a x P' y p. {x,y} \<inter> Psupp p = {} \<Longrightarrow> a \<notin> {x,y} \<Longrightarrow>
     trans P (Bout a x P') \<Longrightarrow> (\<forall>p'. \<phi> p' P (Bout a x P')) \<Longrightarrow> y \<notin> {a, x} \<Longrightarrow> x \<notin> {a} \<union> FFVars P \<Longrightarrow>
-    \<phi> p (Res y P) (Bout a x (Res y P'))" 
-and Par1: 
-"\<And>P1 act P1' P2 p. bvars act \<inter> (Psupp p \<union> fvars act) = {} \<Longrightarrow> 
+    \<phi> p (Res y P) (Bout a x (Res y P'))"
+and Par1:
+"\<And>P1 act P1' P2 p. bvars act \<inter> (Psupp p \<union> fvars act) = {} \<Longrightarrow>
     trans P1 (Cmt act P1') \<Longrightarrow>
     (\<forall>p'. \<phi> p' P1 (Cmt act P1')) \<Longrightarrow>
-    bvars act \<inter> FFVars P1 = {} \<Longrightarrow> 
-    bvars act \<inter> FFVars P2 = {} \<Longrightarrow> 
+    bvars act \<inter> FFVars P1 = {} \<Longrightarrow>
+    bvars act \<inter> FFVars P2 = {} \<Longrightarrow>
     \<phi> p (Par P1 P2) (Cmt act (Par P1' P2))"
-and Com1: 
-"\<And>P1 a x P1' P2 P2' p. 
+and Com1:
+"\<And>P1 a x P1' P2 P2' p.
     trans P1 (Finp a x P1') \<Longrightarrow>
-    (\<forall>p'. \<phi> p' P1 (Finp a x P1')) \<Longrightarrow> 
-    trans P2 (Fout a x P2') \<Longrightarrow> 
-    (\<forall>p'. \<phi> p' P2 (Fout a x P2')) \<Longrightarrow> 
+    (\<forall>p'. \<phi> p' P1 (Finp a x P1')) \<Longrightarrow>
+    trans P2 (Fout a x P2') \<Longrightarrow>
+    (\<forall>p'. \<phi> p' P2 (Fout a x P2')) \<Longrightarrow>
     \<phi> p (Par P1 P2) (Tau (Par P1' P2'))"
-and Close1: 
-"\<And>P1 a x P1' P2 P2' p. x \<notin> Psupp p \<Longrightarrow> x \<notin> FFVars P2 \<Longrightarrow> 
+and Close1:
+"\<And>P1 a x P1' P2 P2' p. x \<notin> Psupp p \<Longrightarrow> x \<notin> FFVars P2 \<Longrightarrow>
     trans P1 (Finp a x P1') \<Longrightarrow>
     (\<forall>p'. \<phi> p' P1 (Finp a x P1')) \<Longrightarrow>
     trans P2 (Bout a x P2') \<Longrightarrow>
-    (\<forall>p'. \<phi> p' P2 (Bout a x P2')) \<Longrightarrow> 
-    x \<notin> {a} \<union> FFVars P1 \<Longrightarrow> 
+    (\<forall>p'. \<phi> p' P2 (Bout a x P2')) \<Longrightarrow>
+    x \<notin> {a} \<union> FFVars P1 \<Longrightarrow>
     \<phi> p (Par P1 P2) (Tau (Res x (Par P1' P2')))"
-shows "\<phi> p P C" 
+shows "\<phi> p P C"
 apply(subgoal_tac "case (P,C) of (P, C) \<Rightarrow> \<phi> p P C")
   subgoal by simp
   subgoal using par tr apply(elim Trans.strong_induct[where R = "\<lambda>p (P,C). \<phi> p P C"])
     subgoal unfolding trans_I by simp
-    subgoal for p v t apply(subst (asm) G_def) 
+    subgoal for p v t apply(subst (asm) G_def)
     unfolding trans_I[symmetric] apply(elim disjE exE)
       subgoal using Inp by auto
       subgoal using Open by auto
-      subgoal for Pa act P' y using ScopeF[of y p act] by (cases act, auto) 
+      subgoal for Pa act P' y using ScopeF[of y p act] by (cases act, auto)
       subgoal using ScopeB by auto
       subgoal for P1 act P1' P2 using Par1[of act] by (cases act, auto)
       subgoal using Com1 by auto
@@ -676,8 +676,8 @@ apply(subgoal_tac "case (P,C) of (P, C) \<Rightarrow> \<phi> p P C")
 
 (* Also inferring equivariance from the general infrastructure: *)
 corollary rrename_pstep:
-assumes f: "bij f" "|supp f| <o |UNIV::var set|" 
-and r: "trans P C" 
+assumes f: "bij f" "|supp f| <o |UNIV::var set|"
+and r: "trans P C"
 shows "trans (rrename f P) (rrename_commit f C)"
 using assms unfolding trans_I using Trans.I_equiv[of "(P,C)" f]
 unfolding Tperm_def isPerm_def by auto
